Another cat1 version, refined fread/fwrite specs

cat/io_specs_cap.v
@@ -1,16 +1,10 @@
 Require Import VST.veric.juicy_extspec.
 Require Import VST.floyd.proofauto.
 Require Export VST.floyd.io_events.
-Require Import ITree.ITree.
-Require Import ITree.Interp.Traces.
-Require Export ITree.Eq.SimUpToTaus.
-(* Import ITreeNotations. *) (* one piece conflicts with subp notation *)
-Notation "t1 >>= k2" := (ITree.bind t1 k2)
-  (at level 50, left associativity) : itree_scope.
+Require Export ITree.ITree.
+Require Export ITree.Eq.Eq.
 Notation "x <- t1 ;; t2" := (ITree.bind t1 (fun x => t2))
   (at level 100, t1 at next level, right associativity) : itree_scope.
-Notation "t1 ;; t2" := (ITree.bind t1 (fun _ => t2))
-  (at level 100, right associativity) : itree_scope.
 Notation "' p <- t1 ;; t2" :=
   (ITree.bind t1 (fun x_ => match x_ with p => t2 end))
 (at level 100, t1 at next level, p pattern, right associativity) : itree_scope.
@@ -18,19 +12,29 @@ Notation "' p <- t1 ;; t2" :=
 Definition stdin := 0%nat.
 Definition stdout := 1%nat.
 
-Axiom enough_console : mpred.
-Axiom has_enough : emp |-- enough_console.
+Inductive IO_cap_event : Type -> Type :=
+| EWriteCap : nat -> byte -> IO_cap_event unit.
 
-Definition putchar_spec :=
+Section specs.
+
+Context {E : Type -> Type} `{IO_cap_event -< E}.
+
+Definition write_cap f c := embed (EWriteCap f c).
+
+Context `{@IO_event nat -< E}.
+
+(* A write_cap event guarantees that the write will succeed, either because the OS has set aside
+  resources sufficient to guarantee it, or because it will block until it succeeds. *)
+Definition putchar_cap_spec :=
   WITH c : byte, k : IO_itree
   PRE [ 1%positive OF tint ]
     PROP ()
     LOCAL (temp 1%positive (Vubyte c))
-    SEP (enough_console; ITREE (write stdout c ;; k))
+    SEP (ITREE (write_cap stdout c ;; k))
   POST [ tint ]
     PROP ()
     LOCAL (temp ret_temp (Vubyte c))
-    SEP (enough_console; ITREE k).
+    SEP (ITREE k).
 
 Definition getchar_spec :=
   WITH k : byte -> IO_itree
@@ -45,9 +49,11 @@ Definition getchar_spec :=
     SEP (ITREE (if eq_dec (Int.signed i) (-1) then (r <- read stdin ;; k r) else k (Byte.repr (Int.signed i)))).
 
 (* Build the external specification. *)
-Definition IO_void_Espec : OracleKind := ok_void_spec (@IO_itree nat).
+Definition IO_void_Espec : OracleKind := ok_void_spec (@IO_itree E).
 
 Definition IO_specs (ext_link : string -> ident) :=
-  [(ext_link "putchar"%string, putchar_spec); (ext_link "getchar"%string, getchar_spec)].
+  [(ext_link "putchar"%string, putchar_cap_spec); (ext_link "getchar"%string, getchar_spec)].
 
 Definition IO_Espec (ext_link : string -> ident) : OracleKind := add_funspecs IO_void_Espec ext_link (IO_specs ext_link).
+
+End specs.
