cat/fio_specs.v
@@ -1,33 +1,44 @@
 Require Import VST.floyd.proofauto.
 Require Import VST.veric.juicy_extspec.
 Require Export VST.floyd.printf.
-Require Import ITree.ITree.
 Require Export ITree.Eq.Eq.
 Require Export ITree.Eq.SimUpToTaus.
-(* Import ITreeNotations. *) (* one piece conflicts with subp notation *)
-Notation "t1 >>= k2" := (ITree.bind t1 k2)
-  (at level 50, left associativity) : itree_scope.
+Require Export ITree.Events.Nondeterminism.
 Notation "x <- t1 ;; t2" := (ITree.bind t1 (fun x => t2))
   (at level 100, t1 at next level, right associativity) : itree_scope.
-Notation "t1 ;; t2" := (ITree.bind t1 (fun _ => t2))
-  (at level 100, right associativity) : itree_scope.
 Notation "' p <- t1 ;; t2" :=
   (ITree.bind t1 (fun x_ => match x_ with p => t2 end))
 (at level 100, t1 at next level, p pattern, right associativity) : itree_scope.
 
-Fixpoint read_list_aux {file_id : Type} f n d : itree (@IO_event file_id) (list byte) :=
-  match n with
-  | O => Ret d
-  | S n' => x <- read f ;; read_list_aux f n' (x :: d)
-  end.
+(* these should be in ITrees *)
+Instance Reflexive_sutt {E R} : RelationClasses.Reflexive (@sutt E R R eq).
+Proof. intro; apply eutt_sutt; reflexivity. Qed.
 
-Definition read_list {file_id : Type} f n : itree (@IO_event file_id) (list byte) := read_list_aux f n [].
+Lemma or_case1 : forall {E R} `{nondetE -< E} a b, sutt eq a (or(R := R) a b).
+Proof.
+  intros; unfold or.
+Admitted.
+
+Lemma or_case2 : forall {E R} `{nondetE -< E} a b, sutt eq b (or(R := R) a b).
+Proof.
+  intros; unfold or.
+Admitted.
 
 Class FileStruct := { abs_file :> FileId; FILEid : ident; reent : ident; f_stdin : ident; f_stdout : ident }.
 
 Instance nat_id : FileId := { file_id := nat; stdin := 0%nat; stdout := 1%nat }.
 
 Section fio_specs.
+
+Context {E : Type -> Type} `{nondetE -< E} `{@IO_event file_id -< E}.
+
+Fixpoint read_list_aux f n d : itree E (list byte) :=
+  match n with
+  | O => Ret d
+  | S n' => or (x <- read f ;; read_list_aux f n' (x :: d)) (read_list_aux f n' d)
+  end.
+
+Definition read_list f n : itree E (list byte) := read_list_aux f n [].
 
 Context {CS : compspecs}.
 Context `{FileStruct}.
@@ -51,6 +62,7 @@ Definition get_reent_spec :=
     LOCAL (temp ret_temp p)
     SEP (reent_struct p).
 
+(* In reality, this might also fail to write all the characters (unless it's a capability version). *)
 Definition fwrite_spec {CS : compspecs} :=
   WITH sh : share, buf : val, len : Z, msg : list byte, sz : Z, count : Z, rest : list val, f : _, fp : val, k : IO_itree
   PRE [ 1%positive OF tptr tvoid, 2%positive OF tuint, 3%positive OF tuint, 4%positive OF tptr (Tstruct FILEid noattr) ]
@@ -71,15 +83,17 @@ Definition fread_spec {CS : compspecs} :=
     PROP (writable_share sh)
     LOCAL (temp 1%positive buf; temp 2%positive (Vint (Int.repr sz));
                temp 3%positive (Vint (Int.repr count)); temp 4%positive fp)
-    SEP (ITREE (r <- read_list f (Z.to_nat (sz * count)) ;; k r); file_at f fp; data_at_ sh (tarray tschar (sz * count)) buf)
+    SEP (ITREE (r <- read_list f (Z.to_nat (sz * count)) ;; k r); file_at f fp;
+           data_at_ sh (tarray tschar (sz * count)) buf)
   POST [ tuint ]
    EX msg : list byte,
     PROP ()
-    LOCAL (temp ret_temp (Vint (Int.repr (sz * count))))
-    SEP (ITREE (k msg); file_at f fp; data_at sh (tarray tschar (sz * count)) (map Vbyte msg) buf).
+    LOCAL (temp ret_temp (Vint (Int.repr (Zlength msg))))
+    SEP (ITREE (k msg); file_at f fp;
+           data_at sh (tarray tschar (sz * count)) (map Vbyte msg ++ repeat Vundef (Z.to_nat (sz * count - Zlength msg))) buf).
 
 (* Build the external specification. *)
-Definition IO_void_Espec : OracleKind := ok_void_spec (@IO_itree nat).
+Definition IO_void_Espec : OracleKind := ok_void_spec (@IO_itree E).
 
 Definition IO_specs {CS : compspecs} (ext_link : string -> ident) :=
   [(ext_link "__getreent"%string, get_reent_spec); (ext_link "fwrite"%string, fwrite_spec);
