cat/io_specs_rollback.v
@@ -4,20 +4,8 @@ Require Export VST.floyd.io_events.
 Require Export ITree.ITree.
 Require Export ITree.Eq.SimUpToTaus.
 Require Export ITree.Events.Nondeterminism.
-(* Import ITreeNotations. *) (* one piece conflicts with subp notation *)
-Notation "t1 >>= k2" := (ITree.bind t1 k2)
-  (at level 50, left associativity) : itree_scope.
-Notation "x <- t1 ;; t2" := (ITree.bind t1 (fun x => t2))
-  (at level 100, t1 at next level, right associativity) : itree_scope.
-Notation "t1 ;; t2" := (ITree.bind t1 (fun _ => t2))
-  (at level 100, right associativity) : itree_scope.
-Notation "' p <- t1 ;; t2" :=
-  (ITree.bind t1 (fun x_ => match x_ with p => t2 end))
-(at level 100, t1 at next level, p pattern, right associativity) : itree_scope.
 
-Definition stdin := 0%nat.
-Definition stdout := 1%nat.
-
+(* these should be in ITrees *)
 Instance Reflexive_sutt {E R} : RelationClasses.Reflexive (@sutt E R R eq).
 Proof. intro; apply eutt_sutt; reflexivity. Qed.
 
@@ -30,6 +18,10 @@ Lemma or_case2 : forall {E R} `{nondetE -< E} a b, sutt eq b (or(R := R) a b).
 Proof.
   intros; unfold or.
 Admitted.
+
+Definition stdin := 0%nat.
+Definition stdout := 1%nat.
+
 Section specs.
 
 Context {E : Type -> Type} `{IO_event(file_id := nat) -< E}.
